Memory/MemoryType.v
@@ -1,0 +1,76 @@
+Require Import Arith ZArith Vrac.Tactics.
+
+Inductive mtyp := i8 | i16 | i32 | i64.
+
+Definition mtyp_eqb κ κ' :=
+  match (κ, κ') with
+  | (i8, i8) => true
+  | (i16, i16) => true
+  | (i32, i32) => true
+  | (i64, i64) => true
+  | _ => false
+  end.
+
+Lemma eq_iff_mtyp_eqb_true :
+  forall κ κ', κ = κ' <-> mtyp_eqb κ κ' = true.
+Proof.
+  intros κ κ'; split; intro H;
+    destruct κ; destruct κ'; subst; now compute.
+Qed.
+
+Lemma mtyp_eqb_refl :
+  forall κ, mtyp_eqb κ κ = true.
+Proof.
+  intros; now apply eq_iff_mtyp_eqb_true.
+Qed.
+
+Lemma mtyp_eqb_sym :
+  forall κ κ', mtyp_eqb κ κ' = mtyp_eqb κ' κ.
+Proof.
+  intros; destruct κ; destruct κ'; trivial.
+Qed.
+
+Lemma mtyp_eqb_neq:
+  forall κ κ', mtyp_eqb κ κ' = false <-> κ <> κ'.
+Proof.
+  intros κ κ'; split; intro H.
+  - contradict H; apply eq_iff_mtyp_eqb_true in H; rewrite H; now intro H'.
+  - apply Bool.not_true_is_false. contradict H.
+    now apply eq_iff_mtyp_eqb_true.
+Qed.
+
+Definition sizeof: mtyp -> Z :=
+  fun type => match type with
+           | i8 => 1%Z
+           | i16 => 2%Z
+           | i32 => 4%Z
+           | i64 => 8%Z
+           end.
+
+Lemma sizeof_pos:
+  forall κ, (0 <= sizeof κ)%Z.
+Proof.
+  now destruct κ.
+Qed.
+
+Ltac simpl_mtyp :=
+  try simpl_eqb;
+  match goal with 
+  | [ |- context [mtyp_eqb ?x ?x ] ] =>
+      rewrite mtyp_eqb_refl; simpl
+  | [ H: context [ mtyp_eqb ?x ?x ] |- _ ] =>
+      rewrite mtyp_eqb_refl in H; simpl in H
+  | [ H: mtyp_eqb ?x ?y = true |- _ ] =>
+      apply eq_iff_mtyp_eqb_true in H; subst
+  | [ Hn: ?x <> ?y |- context [mtyp_eqb ?x ?y ] ] =>
+      apply mtyp_eqb_neq in Hn; rewrite Hn; simpl
+  | [ Hn: ?x <> ?y, H: context [ mtyp_eqb ?x ?y ] |- _ ] =>
+      apply mtyp_eqb_neq in Hn; rewrite Hn in H; simpl in H
+  | [ Hn: ?y <> ?x |- context [mtyp_eqb ?x ?y ] ] =>
+      apply mtyp_eqb_neq in Hn; rewrite mtyp_eqb_sym in Hn; rewrite Hn;
+      apply mtyp_eqb_neq in Hn; simpl
+  | [ Hn: ?y <> ?x, H: context [ mtyp_eqb ?x ?y ] |- _ ] =>
+      apply mtyp_eqb_neq in Hn; rewrite mtyp_eqb_sym in Hn; rewrite Hn in H;
+      apply mtyp_eqb_neq in Hn; simpl in H
+  end.
+
