Memory/Option.v
@@ -1,0 +1,8 @@
+Notation "'⎣' v '⎦'" := (Some v).
+Notation "'ϵ'" := (None).
+
+Definition is_ϵ {A} (v: option A) :=
+  match v with
+  | ϵ => true
+  | _ => false
+  end.
