Memory/Tactics.v
@@ -1,0 +1,203 @@
+Require Import Arith ZArith List Bool.
+
+Ltac destruct_and_hyp := 
+  match goal with
+  | [ H : (_ && _)%bool = true |- _ ] =>
+      apply andb_prop in H;
+      let H1 := fresh H in
+      let H2 := fresh H in 
+      destruct H as [H1 H2]
+  | [ H : (_ && _)%bool = false |- _ ] =>
+      apply Bool.andb_false_iff in H;
+      let HH := fresh H in
+      destruct H as [HH | HH]
+  | [ H : _ /\ _ |- _ ] =>
+      let H1 := fresh H in
+      let H2 := fresh H in 
+      destruct H as [H1 H2]
+  end.
+
+Ltac destruct_or_hyp := 
+  match goal with
+  | [ H : (_ || _)%bool = true |- _ ] =>
+      apply orb_prop in H;
+      destruct H as [H | H]
+  | [ H : (_ || _)%bool = false |- _ ] =>
+      apply Bool.orb_false_iff in H;
+      let HH := fresh H in
+      destruct H as [H1 H2]
+  | [ H : _ \/ _ |- _ ] =>
+      destruct H as [H|H]
+  end.
+
+Ltac destruct_and_goal :=
+  match goal with 
+  | [ |- (_ && _)%bool = true ] =>
+        apply andb_true_intro; split
+  | [ |- _ /\ _ ] => split 
+  end.
+
+Ltac Zleb :=
+  match goal with
+  | [ H: (_ <=? _) = true |- _ ] => apply Z.leb_le in H
+  | [ H: (_ <=? _) = false |- _ ] => apply Z.leb_nle in H
+  | [ |- (_ <=? _) = true ] => apply Z.leb_le 
+  | [ |- (_ <=? _) = false ] => apply Z.leb_nle 
+  end.
+      
+Ltac Zltb :=
+  match goal with
+  | [ H: (_ <? _) = true |- _ ] => apply Z.ltb_lt in H
+  | [ H: (_ <? _) = false |- _ ] => apply Z.ltb_nlt in H
+  | [ |- (_ <? _) = true ] => apply Z.ltb_lt
+  | [ |- (_ <? _) = false ] => apply Z.ltb_nlt 
+  end.
+
+Ltac leb :=
+  match goal with
+  | [ H: (_ <=? _)%nat = true |- _ ] => apply Nat.leb_le in H
+  | [ H: (_ <=? _)%nat = false |- _ ] => apply Nat.leb_nle in H
+  | [ |- (_ <=? _)%nat = true ] => apply Nat.leb_le 
+  | [ |- (_ <=? _)%nat = false ] => apply Nat.leb_nle 
+  end.
+
+Ltac ltb :=
+  match goal with
+  | [ H: (_ <? _)%nat = true |- _ ] => apply Nat.ltb_lt in H
+  | [ H: (_ <? _)%nat = false |- _ ] => apply Nat.ltb_nlt in H
+  | [ |- (_ <? _)%nat = true ] => apply Nat.ltb_lt
+  | [ |- (_ <? _)%nat = false ] => apply Nat.ltb_nlt 
+  end.
+
+Ltac negb :=
+  match goal with
+  | [ H: negb _ = true |- _ ] => apply Bool.negb_true_iff in H
+  | [ H: negb _ = false |- _ ] => apply Bool.negb_false_iff in H
+  | [ |- negb _ = true ] => apply Bool.negb_true_iff
+  | [ |- negb _ = false ] => apply Bool.negb_false_iff
+  end.
+
+Ltac imp :=
+  match goal with
+  | [ |- _ <-> _ ] => split; let H := fresh "H" in intro H
+  end.
+
+Ltac simpl_eqb:=
+  match goal with
+  | [ |- context [ Nat.eqb ?x ?x ] ] =>
+      rewrite Nat.eqb_refl; simpl
+  | [ H: context [ Nat.eqb ?x ?x ] |- _ ] =>
+      rewrite Nat.eqb_refl in H; simpl in H
+  | [ |- context [ Z.eqb ?x ?x ] ] =>
+      rewrite Z.eqb_refl; simpl
+  | [ H: context [ Z.eqb ?x ?x ] |- _ ] =>
+      rewrite Z.eqb_refl in H; simpl in H
+  | [ H: context [ Nat.eqb ?x ?x ] |- _ ] =>
+      rewrite Nat.eqb_refl in H; simpl in H
+  | [ H: Nat.eqb ?x ?y = true |- _ ] =>
+      apply Nat.eqb_eq in H; subst 
+  | [ H: Z.eqb ?x ?y = true |- _ ] =>
+      apply Z.eqb_eq in H; subst
+
+  | [ Hn: ?x = ?y, He: Nat.eqb ?x ?y = false |- _ ] => 
+      apply Nat.eqb_neq in He; rewrite Hn in He; simpl
+  | [ Hn: ?y = ?x, He: Nat.eqb ?x ?y = false |- _ ] =>
+      apply Nat.eqb_neq in He; rewrite Hn in He; simpl
+                                                                          
+  | [ Hn: ?x <> ?y, H: context [ Nat.eqb ?x ?y ] |- _ ] =>
+      apply Nat.eqb_neq in Hn; rewrite Hn in H; simpl in H
+  | [ Hn: ?x <> ?y |- context [ Nat.eqb ?x ?y ] ] =>
+      apply Nat.eqb_neq in Hn; rewrite Hn; simpl
+  | [ Hn: ?x <> ?y, H: context [ Nat.eqb ?x ?y ] |- _ ] =>
+      apply Nat.eqb_neq in Hn; rewrite Hn in H; simpl in H
+  | [ Hn: ?x <> ?y |- context [ Z.eqb ?x ?y ] ] =>
+      apply Z.eqb_neq in Hn; rewrite Hn; simpl
+  | [ Hn: ?x <> ?y, H: context [ Z.eqb ?x ?y ] |- _ ] =>
+      apply Z.eqb_neq in Hn; rewrite Hn in H; simpl in H
+                                                            
+  | [ Hn: ?y <> ?x |- context [ Nat.eqb ?x ?y ] ] =>
+      apply Nat.eqb_neq in Hn; rewrite Nat.eqb_sym in Hn; rewrite Hn;
+      apply Nat.eqb_neq in Hn; simpl
+  | [ Hn: ?y <> ?x, H: context [ Nat.eqb ?x ?y ] |- _ ] =>
+      apply Nat.eqb_neq in Hn; rewrite Nat.eqb_sym in Hn; rewrite Hn in H;
+      apply Nat.eqb_neq in Hn; simpl in H
+  | [ Hn: ?y <> ?x |- context [ Z.eqb ?x ?y ] ] =>
+      apply Z.eqb_neq in Hn; rewrite Z.eqb_sym in Hn; rewrite Hn;
+      apply Z.eqb_neq in Hn; simpl
+  | [ Hn: ?y <> ?x, H: context [ Z.eqb ?x ?y ] |- _ ] =>
+      apply Z.eqb_neq in Hn; rewrite Z.eqb_sym in Hn; rewrite Hn in H;
+      apply Z.eqb_neq in Hn; simpl in H
+  end; simpl in *.
+
+Ltac simpl_if :=
+  match goal with
+  | [ Hcond: ?cond = true, 
+        H: context [if ?cond then _ else _] |- _] =>
+      rewrite Hcond in H; simpl in H
+  | [ Hcond: ?cond = false, 
+        H: context [if ?cond then _ else _] |- _] =>
+      rewrite Hcond in H; simpl in H
+  | [ Hcond: true = ?cond, 
+        H: context [if ?cond then _ else _] |- _] =>
+      rewrite Hcond in H; simpl in H
+  | [ Hcond: false = ?cond, 
+        H: context [if ?cond then _ else _] |- _] =>
+      rewrite Hcond in H; simpl in H
+  | [ Hcond: ?cond = true |-  
+        context [if ?cond then _ else _] ] =>
+      rewrite Hcond; simpl
+  | [ Hcond: ?cond = false |-
+        context [if ?cond then _ else _] ] =>
+      rewrite Hcond; simpl
+  | [ Hcond: true = ?cond |-
+        context [if ?cond then _ else _] ] =>
+      rewrite Hcond; simpl
+  | [ Hcond: false = ?cond |- 
+        context [if ?cond then _ else _] ] =>
+      rewrite Hcond; simpl
+  | [ H: context [if ?cond then _ else _] |- _] =>
+      case_eq(cond);
+      let HH := fresh "H" in intro HH; rewrite HH in H; simpl in *
+  | [ |- context [if ?cond then _ else _] ] =>
+      case_eq(cond);
+      let HH := fresh "H" in intro HH; try rewrite HH; simpl in *
+  end.
+
+Ltac clean_inv H :=
+  inversion H; subst; clear H; simpl in *.
+
+Ltac existsb_true :=
+  match goal with
+  | [ H: existsb (Nat.eqb _) _ = true |- _ ] =>
+      apply existsb_exists in H;
+      let x := fresh "x" in
+      let Hin := fresh "Hin" in
+      let Heq := fresh "Heq" in 
+      destruct H as [x [Hin Heq]]
+  | [ H: In ?x ?l |- existsb (Nat.eqb _) ?l = true ] => 
+      apply existsb_exists;
+      exists x; split; auto; now simpl_eqb
+  end.
+
+Ltac existsb_false :=
+  match goal with
+  | [ H : existsb (Nat.eqb ?x) ?l = false |- not(In ?x ?l) ] =>
+      apply Bool.not_true_iff_false in H;
+      contradict H;
+      existsb_true
+  | [ H : not(In ?x ?l) |- existsb (Nat.eqb ?x) ?l = false ] =>
+      apply Bool.not_true_iff_false;
+      contradict H;
+      existsb_true; now simpl_eqb
+  end.
+
+Ltac by_contradiction :=
+  match goal with
+  | [ H: ?hyp, H': ~?hyp |- _ ] => now contradict H
+  | [ H: ~(?x = ?x)  |- _ ] => now contradict H
+  | [ H: ?x = true, H': ?x = false  |- _ ] =>
+      rewrite H in H'; discriminate
+  | [ H1: In ?x ?l, H2: existsb (Nat.eqb ?x) ?l = false |- _ ] =>
+      apply Bool.not_true_iff_false in H2;
+      contradict H2; existsb_true
+  end.
